formal/SkLean/Ast3.lean
@@ -36,14 +36,14 @@ def arrow : Expr := SKM[((S (K ((S (K S)) K))) K)]
 def t_in  : Expr := SKM[((S ((S K) K)) (K K))]
 def t_out : Expr := SKM[((S i) (K (K i)))]
 
-def t_k : Expr := SKM[((S ((S (K ((S (K ((S (K S)) K))) K))) ((S (K M)) ((S K) K)))) ((S ((S (K S)) ((S ((S (K S)) ((S (K K)) (K ((S (K ((S (K S)) K))) K))))) ((S ((S (K S)) ((S (K K)) (K M)))) ((S ((S (K S)) (K K))) (K K)))))) ((S ((S (K S)) ((S (K K)) (K M)))) ((S (K K)) ((S K) K)))))]
-def t_s : Expr := SKM[((S ((S (K ((S (K ((S (K S)) K))) K))) ((S (K M)) ((S K) K)))) ((S ((S (K S)) ((S ((S (K S)) ((S (K K)) (K ((S (K ((S (K S)) K))) K))))) ((S ((S (K S)) ((S (K K)) (K M)))) ((S ((S (K S)) (K K))) (K K)))))) ((S ((S (K S)) ((S ((S (K S)) ((S (K K)) (K S)))) ((S ((S (K S)) ((S ((S (K S)) ((S (K K)) (K S)))) ((S ((S (K S)) ((S (K K)) (K K)))) ((S (K K)) (K ((S (K ((S (K S)) K))) K))))))) ((S ((S (K S)) ((S ((S (K S)) ((S (K K)) (K S)))) ((S ((S (K S)) ((S (K K)) (K K)))) ((S (K K)) (K M)))))) ((S ((S (K S)) ((S ((S (K S)) ((S (K K)) (K S)))) ((S (K K)) (K K))))) ((S (K K)) (K K)))))))) ((S ((S (K S)) ((S ((S (K S)) ((S (K K)) (K S)))) ((S ((S (K S)) ((S (K K)) (K K)))) ((S (K K)) (K ((S ((S K) K)) (K (K ((S K) K)))))))))) ((S ((S (K S)) ((S ((S (K S)) ((S (K K)) (K S)))) ((S ((S (K S)) ((S ((S (K S)) ((S (K K)) (K S)))) ((S ((S (K S)) ((S (K K)) (K K)))) ((S (K K)) (K ((S ((S K) K)) (K (K ((S K) K)))))))))) ((S ((S (K S)) ((S ((S (K S)) ((S (K K)) (K S)))) ((S ((S (K S)) ((S ((S (K S)) ((S (K K)) (K S)))) ((S ((S (K S)) ((S (K K)) (K K)))) ((S (K K)) (K M)))))) ((S ((S (K S)) ((S (K K)) (K K)))) ((S (K K)) ((S K) K))))))) ((S ((S (K S)) ((S ((S (K S)) ((S (K K)) (K S)))) ((S (K K)) (K K))))) ((S (K K)) (K K)))))))) ((S ((S (K S)) ((S ((S (K S)) ((S (K K)) (K S)))) ((S ((S (K S)) ((S (K K)) (K K)))) ((S (K K)) (K ((S ((S K) K)) (K (K ((S K) K)))))))))) ((S ((S (K S)) ((S ((S (K S)) ((S (K K)) (K S)))) ((S ((S (K S)) ((S ((S (K S)) ((S (K K)) (K S)))) ((S ((S (K S)) ((S (K K)) (K K)))) ((S (K K)) (K M)))))) ((S ((S (K S)) ((S (K K)) (K K)))) ((S ((S (K S)) (K K))) (K K))))))) ((S ((S (K S)) ((S ((S (K S)) ((S (K K)) (K S)))) ((S (K K)) (K K))))) ((S (K K)) (K K))))))))))]
-def t_m : Expr := SKM[((S ((S (K ((S (K ((S (K S)) K))) K))) ((S (K M)) ((S K) K)))) ((S (K M)) ((S (K M)) ((S K) K))))]
+def t_k : Expr := SKM[((S ((S (K S)) M)) K)]
+def t_s : Expr := SKM[((S ((S (K S)) ((S ((S (K S)) (K (K S)))) M))) S)]
+def t_m : Expr := SKM[((S M) M)]
 
 inductive is_eval_once : Expr → Expr → Prop
   | k      : is_eval_once SKM[((K x) _y)] x
   | s      : is_eval_once SKM[(((S x) y) z)] SKM[((x z) (y z))]
-  | m_call : is_eval_once SKM[(M (lhs rhs))] SKM[(t_out ((M lhs) rhs))]
+  | m_call : is_eval_once SKM[(M (lhs rhs))] SKM[((M lhs) rhs)]
   | m_k    : is_eval_once SKM[(M K)] t_k
   | m_s    : is_eval_once SKM[(M S)] t_s
   | m_m    : is_eval_once SKM[(M M)] t_m
@@ -66,40 +66,30 @@ inductive is_normal_n : ℕ → Expr → Expr → Prop
   | stuck : (¬(∃ e', is_eval_once e e'))                 → is_normal_n 0 e e
   | succ  : is_eval_once e e' → is_normal_n n e' e_final → is_normal_n n.succ e e_final
 
+def subtree_is_in (e in_e : Expr) : Prop :=
+  e == in_e ∨
+    match in_e with
+      | SKM[(lhs rhs)] => subtree_is_in e lhs ∨ subtree_is_in e rhs
+      | _ => false
+
 inductive valid_judgment_hard : Expr → Expr → Prop
-  | call    : is_eval_once SKM[(M (lhs rhs))] t_output
-    → beta_eq SKM[(t_in ((M lhs) rhs))] SKM[(M rhs)]
-    → valid_judgment_hard SKM[(lhs rhs)] SKM[(M (lhs rhs))]
-  | s       : valid_judgment_hard SKM[S] t_s
-  | k       : valid_judgment_hard SKM[K] t_k
-  | m       : valid_judgment_hard SKM[M] t_m
-  | beta_eq : valid_judgment_hard e t₁
-    → beta_eq t₁ t₂
-    → valid_judgment_hard e t₂
+  | m : beta_eq SKM[(M e)] t
+    → ¬ subtree_is_in e t
+    → valid_judgment_hard e t
 
 namespace valid_judgment_hard
 
-lemma imp_m_eval : valid_judgment_hard e t → _root_.beta_eq SKM[(M e)] t := by
-  intro h_t
-  induction h_t
-  apply _root_.beta_eq.rfl
-  apply _root_.beta_eq.eval
-  apply is_eval_once.m_s
-  apply _root_.beta_eq.eval
-  apply is_eval_once.m_k
-  apply _root_.beta_eq.eval
-  apply is_eval_once.m_m
-  case beta_eq e t₁ t₂ h_t₁ h_beq ih =>
-    apply _root_.beta_eq.trans
-    exact ih
-    exact h_beq
+lemma imp_m_eval : valid_judgment_hard e t → _root_.beta_eq SKM[(M e)] t :=
+  fun h_t =>
+    match h_t with
+      | .m h_beq _ => h_beq
 
 end valid_judgment_hard
 
 namespace beta_eq
 
 @[simp]
-lemma m_distributes : beta_eq SKM[(t_out ((M lhs) rhs))] SKM[(M (lhs rhs))] := by
+lemma m_distributes : beta_eq SKM[((M lhs) rhs)] SKM[(M (lhs rhs))] := by
   apply beta_eq.symm
   apply beta_eq.eval
   apply is_eval_once.m_call
